FA2 safety proof back again

examples/fac_master/tzwrap/fa2/multi_asset/FA2_Multi_Asset.v
@@ -1,5 +1,7 @@
 Require Import Blockchain.
 From ConCert.Examples Require Import FA2Interface.
+From ConCert.Utils Require Import Extras.
+From ConCert.Execution Require Import InterContractCommunication.
 Require Import FA2InterfaceOwn.
 Require Import RecordUpdate.
 Require Import ContractCommon.
@@ -19,6 +21,7 @@ Require Import FA2_Operator_Lib.
 Require Import FSets.
 Require Import FMapList.
 Require Import Psatz.
+Require Import TokenAdmin.
 Import ListNotations.
 
 
@@ -339,4 +342,108 @@ Proof.
     setoid_rewrite H. destruct (v <? amount) eqn: E; try easy. rewrite N.ltb_ge in E. easy.
 Qed.
 
+(**----------------- FA2_Multi_Asset -----------------**)
+Definition sum_tx (txs : list MintBurnTx) (id : token_id): Z :=
+    fold_right 
+    (fun (tx : MintBurnTx) (acc : Z) => 
+        (
+            if tx.(mint_burn_token_id) =? id
+            then (acc + (Z.of_N tx.(mint_burn_amount)))%Z
+            else 0%Z
+        )
+        )
+    0%Z txs.
+
+Definition mint_or_burn (id : token_id) (msg : option MultiAssetParam) : Z :=
+    match msg with
+    | Some m =>
+        match m with
+        | Tokens (param) =>
+            match param with 
+            | MintTokens mint_param => sum_tx mint_param id
+            | BurnTokens mint_param => (sum_tx mint_param id) * (-1)
+            end
+        | _ => 0
+        end
+    | _ => 0
+    end.
+
+Lemma init_total_supply_correct {chain ctx setup state fa2_token_id total_supply} :
+    FMap.find fa2_token_id state.(fa2_assets).(token_total_supply) = Some total_supply ->
+    fa2_init chain ctx setup = Some state ->
+    total_supply = 0.
+Proof.
+    contract_simpl fa2_receive fa2_init. Admitted.
+
+Lemma assets_endpoint_does_not_change_minter {prev_state next_state acts chain ctx param} :
+    fa2_receive chain ctx prev_state (Some (Assets param)) = Some (next_state, acts) ->
+    prev_state.(fa2_admin).(tas_minter) = next_state.(fa2_admin).(tas_minter).
+Proof.
+    intros; now contract_simpl fa2_receive fa2_init.
+Qed. 
+
+Lemma balance_of_preserves_total_supply {prev_state next_state acts chain ctx param} :
+    fa2_receive chain ctx prev_state (Some (Assets (Balance_of (param)))) = Some (next_state, acts) ->
+    prev_state.(fa2_assets).(token_total_supply) = next_state.(fa2_assets).(token_total_supply).
+Proof.
+    intros. contract_simpl fa2_receive fa2_init.
+Qed. 
+
+Lemma update_operators_preserves_total_supply {prev_state next_state acts chain ctx param} :
+    fa2_receive chain ctx prev_state (Some (Assets (Update_operators (param)))) = Some (next_state, acts) ->
+    prev_state.(fa2_assets).(token_total_supply) = next_state.(fa2_assets).(token_total_supply).
+Proof.
+    intros. contract_simpl fa2_receive fa2_init.
+Qed. 
+
+Lemma assets_endpoint_preserves_total_supply {prev_state next_state acts chain ctx param} :
+    fa2_receive chain ctx prev_state (Some (Assets param)) = Some (next_state, acts) ->
+    prev_state.(fa2_assets).(token_total_supply) = next_state.(fa2_assets).(token_total_supply).
+Proof.
+    intros. contract_simpl fa2_receive fa2_init. destruct param.
+    - inversion H1. destruct (transfer ctx transfers default_operator_validator (fa2_assets prev_state)) in H2.
+     now inversion H2.
+
+Qed. 
+
+Lemma set_admin_preserves_total_supply {prev_state next_state acts chain ctx addr} :
+    fa2_receive chain ctx prev_state (Some (Admin (Token_admin (Set_admin addr)))) = Some (next_state, acts) ->
+    prev_state.(fa2_assets).(token_total_supply) = next_state.(fa2_assets).(token_total_supply).
+Proof.
+    intros. contract_simpl fa2_receive fa2_init.
+Qed.
+
+Lemma set_admin_does_not_change_minter {prev_state next_state chain ctx addr acts} :
+    fa2_receive chain ctx prev_state (Some (Admin (Token_admin (Set_admin addr)))) = Some (next_state, acts) ->
+    prev_state.(fa2_admin).(tas_minter) = next_state.(fa2_admin).(tas_minter).
+Proof.
+    intros. contract_simpl fa2_receive fa2_init. unfold set_admin.
+    cbn. unfold fail_if_not_admin in H. destruct_address_eq; try easy.
+Qed. 
+
+Lemma fa2_correct : forall bstate caddr fa2_token_id total_supply (trace: ChainTrace empty_state bstate),
+    env_contracts bstate caddr = Some (FA2_contract : WeakContract) ->
+    exists cstate depinfo inc_calls,
+        contract_state bstate caddr = Some cstate /\
+        deployment_info Setup trace caddr = Some depinfo /\
+        incoming_calls MultiAssetParam trace caddr = Some inc_calls /\
+        (
+        FMap.find fa2_token_id cstate.(fa2_assets).(token_total_supply) = Some total_supply ->
+        sumZ (fun callInfo => mint_or_burn fa2_token_id callInfo.(call_msg)) (filter (callFrom cstate.(fa2_admin).(tas_minter)) inc_calls) = Z.of_N total_supply
+        ).
+Proof.
+    contract_induction;
+    intros; auto.
+    - intros. cbn in *. eapply init_total_supply_correct in init_some; now eauto.
+    - unfold callFrom. unfold receive in receive_some. simpl in *. destruct msg; try easy. destruct m. destruct param. 
+        + erewrite <- transfer_preserves_total_supply in H; eauto. erewrite <- assets_endpoint_does_not_change_minter; eauto.
+        destruct_address_eq; now apply IH.
+        + erewrite <- balance_of_preserves_total_supply in H; eauto. erewrite <- assets_endpoint_does_not_change_minter; eauto.
+        destruct_address_eq; now apply IH.
+        + erewrite <- update_operators_preserves_total_supply in H; eauto. erewrite <- assets_endpoint_does_not_change_minter; eauto.  
+        destruct_address_eq; now apply IH.
+        + destruct param. destruct tokenAdmin.
+            -- erewrite <- set_admin_preserves_total_supply in H; eauto. erewrite <- set_admin_does_not_change_minter; eauto.
+            destruct_address_eq; now apply IH.
+            -- 
 End FA2_Multi_Asset.
